---
title: "HW05"
author: "Chongdan Pan"
date: "2022/3/2"
output: html_document
---

```{r setup, include=FALSE}
knitr::opts_chunk$set(echo = TRUE)
```

Since the random variable used for each probability function is clearly represented in the arguments, I'm omitting the subscription of the functions.

### 5.1 Derive the identity
Based on the definition of Markov process and conditional probability, we have
$$
f(x_{0:N})=f(x_N|x_{0:N-1})f(x_{0:N-1})=f(x_N|x_{N-1})f(x_{0:N-1})
$$
By applying the formula recursively, we have 
$$
f(x_{0:N})=f(x_N|x_{N-1})f(x_{0:N-1})=f(x_0)\prod_{t=1}^Nf(x_t|x_{t-1})
$$

### 5.2 Derive the prediction 

Based on Bayies theorem, we have 


$$
f_(x_n|y^*_{1:n-1})=\int_{x_{n-1}}f_(x_n,x_{n-1}|y^*_{1:n-1})\mathrm dx_{n-1}=\\\int f(x_n|x_{n-1},y^*_{1:n-1})f(x_{n-1}|y^*_{1:n-1})\mathrm dx_{n-1}
$$

Since $f(x_n|x_{n-1},y^*_{1:n-1})=f(x_n|x_{n-1})$

we have
$$
f(x_n|y^*_{1:n-1})=\int f(x_{n-1}|y^*_{1:n-1})f(x_n|x_{n-1})\mathrm dx_{n-1}
$$

### 5.3 Derive the filtering

- For [P5]

$$
f(x_n|y^*_{1:n})=\frac{f(x_n,y^*_n|y^*_{1:n-1})}{f(y^*_n|y^*_{1:n-1})}=\frac{f(y^*_n|x_n,y^*_{1:n-1})f(x_n|y^*_{1:n-1})}{f(y^*_n|y^*_{1:n-1})}
$$

Since we have $f(y^*_n|x_n,y^*_{1:n-1})=f(y^*_n|x_n)$
$$
f(x_n|y^*_{1:n})=\frac{f(x_n|y^*_{1:n-1})f(y^*_n|x_n)}{f(y^*_n|y^*_{1:n-1})}
$$

- For [P6]

$$
f(y^*_n|y^*_{1:n-1})=\int f(y^*_n|x_n,y^*_{1:n-1})f(x_n|y^*_{1:n-1})\mathrm dx_n
$$

Since $f(y^*_n|x_n,y^*_{1:n-1})=f(y^*_n|x_n)$

We have 
$$
f(y^*_n|y^*_{1:n-1})=\int f(x_n|y^*_{1:n-1})f(y^*_n|x_n)\mathrm dx_n
$$

### 5.4 Derive the backward recursion

- For [P7]

$$f(y^*_{n:N}|x_n)=f(y^*_n|y^*_{n+1:N},x_n)f(y^*_{n+1:N}|x_n)$$

Since $f(y^*_n|y^*_{n+1:N},x_n)=f(y^*_n|x_n)$

We have 

$$
f(y^*_{n:N}|x_n)=f(y^*_n|x_n)f(y^*_{n+1:N}|x_n)
$$

- For [P8]

$$
f(y^*_{n+1:N}|x_n)=\int f(y^*_{n+1:N}|x_n,x_{n+1})f(x_{n+1}|x_n)\mathrm d x_{n+1}
$$

Since $f(y^*_{n+1:N}|x_n,x_{n+1})=f(y^*_{n+1:N}|x_{n+1})$

we have 

$$
f(y^*_{n+1:N}|x_n)=\int f(y^*_{n+1:N}|x_{n+1})f(x_{n+1}|x_n)\mathrm d x_{n+1}
$$

### 5.5 Derive the smoothing

$$
f(x_n|y^*_{1:N})=\frac{f(x_n,y^*_{n:N}|y^*_{1:n-1})}{f(y^*_{n:N}|y^*_{1:n-1})}=\frac{f(x_n|y^*_{1:n-1})f(y^*_{n:N}|x_n,y^*_{1:n-1})}{f(y^*_{n:N}|y^*_{1:n-1})}
$$

Since $f(y_{n:N}|x_n,y_{1:n-1})=f(y_{n:N}|x_n)$

We have 
$$
f(x_n|y^*_{1:N})=\frac{f(x_n|y^*_{1:n-1})f(y^*_{n:N}|x_n)}{f(y^*_{n:N|y^*_{1:n-1}})}
$$

### Refernce

- [Slides about Chapter 10](https://ionides.github.io/531w22/10/index.html)